Merkle tree: working on the correctness of high-level design

secure_api/merkle_tree/MerkleTree.New.High.Correct.fst
@@ -129,6 +129,16 @@ let hash_seq_spec_rel j n olds hs smt =
   S.equal (hash_seq_lift (S.append olds hs))
           (S.slice smt 0 j)
 
+val hash_seq_spec_rel_equiv:
+  j:nat -> n:nat{j <= pow2 n} ->
+  olds:hash_seq ->
+  hs:hash_seq{S.length hs = j - S.length olds} ->
+  smt1:MTS.merkle_tree n -> smt2:MTS.merkle_tree n ->
+  Lemma (requires (hash_seq_spec_rel j n olds hs smt1 /\
+                  S.equal (S.slice smt1 0 j) (S.slice smt2 0 j)))
+        (ensures (hash_seq_spec_rel j n olds hs smt2))
+let hash_seq_spec_rel_equiv j n olds hs smt1 smt2 = ()
+
 val hash_ss_length_spec:
   j:nat -> n:nat{j <= pow2 n} ->
   olds:hash_ss{S.length olds = n} ->
@@ -136,7 +146,7 @@ val hash_ss_length_spec:
   GTot Type0
 let rec hash_ss_length_spec j n olds hs =
   if n = 0 then true
-  else (S.length (S.head hs) = j - S.length (S.head olds) /\
+  else (S.length (S.append (S.head olds) (S.head hs)) = j /\
        hash_ss_length_spec (j / 2) (n - 1) (S.tail olds) (S.tail hs))
 
 val hash_ss_spec_rel:
@@ -151,12 +161,36 @@ let rec hash_ss_spec_rel j n olds hs smt =
        hash_ss_spec_rel (j / 2) (n - 1) 
          (S.tail olds) (S.tail hs) (mt_next_lv smt))
 
+val hash_ss_spec_rel_equiv:
+  j:nat -> n:nat{j <= pow2 n} ->
+  olds:hash_ss{S.length olds = n} ->
+  hs:hash_ss{S.length hs = n /\ hash_ss_length_spec j n olds hs} ->
+  smt1:MTS.merkle_tree n -> smt2:MTS.merkle_tree n ->
+  Lemma (requires (hash_ss_spec_rel j n olds hs smt1 /\
+                  S.equal (S.slice smt1 0 j) (S.slice smt2 0 j)))
+        (ensures (hash_ss_spec_rel j n olds hs smt2))
+let rec hash_ss_spec_rel_equiv j n olds hs smt1 smt2 =
+  if n = 0 then ()
+  else (mt_next_lv_equiv j n smt1 smt2;
+       hash_ss_spec_rel_equiv (j / 2) (n - 1) (S.tail olds) (S.tail hs)
+                              (mt_next_lv smt1) (mt_next_lv smt2))
+
 val hash_seq_lift_to_spec:
   fhs:hash_seq ->
   n:nat{S.length fhs <= pow2 n} ->
   GTot (MTS.merkle_tree n)
 let hash_seq_lift_to_spec fhs n =
   S.append (hash_seq_lift fhs) (create_pads (pow2 n - S.length fhs))
+
+val hash_seq_lift_to_spec_slice_eq:
+  fhs1:hash_seq -> fhs2:hash_seq ->
+  n:nat{S.length fhs1 <= pow2 n && S.length fhs2 <= pow2 n} ->
+  i:nat{i <= S.length fhs1 && i <= S.length fhs2} ->
+  Lemma (requires (S.equal (S.slice fhs1 0 i) (S.slice fhs2 0 i)))
+        (ensures (S.equal (S.slice (hash_seq_lift_to_spec fhs1 n) 0 i)
+                          (S.slice (hash_seq_lift_to_spec fhs2 n) 0 i)))
+let hash_seq_lift_to_spec_slice_eq fhs1 fhs2 n i =
+  admit ()
 
 val hash_ss_spec_:
   j:nat -> n:nat{n > 0 && j <= pow2 n} ->
@@ -166,6 +200,25 @@ val hash_ss_spec_:
 let hash_ss_spec_ j n olds hs =
   hash_ss_spec_rel j n olds hs 
     (hash_seq_lift_to_spec (S.append (S.head olds) (S.head hs)) n)
+
+val hash_ss_spec_rec:
+  j:nat -> n:nat{n > 1 && j <= pow2 n} ->
+  olds:hash_ss{S.length olds = n} ->
+  hs:hash_ss{S.length hs = n /\ hash_ss_length_spec j n olds hs} ->
+  Lemma (requires (hash_ss_spec_ j n olds hs))
+        (ensures (hash_ss_spec_ (j / 2) (n - 1) (S.tail olds) (S.tail hs)))
+let hash_ss_spec_rec j n olds hs =
+  let spec_base = hash_seq_lift_to_spec (S.append (S.head olds) (S.head hs)) n in
+  assert (hash_seq_spec_rel (j / 2) (n - 1)
+           (S.head (S.tail olds)) (S.head (S.tail hs)) (mt_next_lv spec_base));
+  assert (S.equal (S.slice (mt_next_lv spec_base) 0 (j / 2))
+                  (S.slice (hash_seq_lift_to_spec
+                             (S.append (S.head (S.tail olds)) 
+                                       (S.head (S.tail hs))) (n - 1)) 0 (j / 2)));
+  hash_ss_spec_rel_equiv (j / 2) (n - 1) (S.tail olds) (S.tail hs)
+    (mt_next_lv spec_base)
+    (hash_seq_lift_to_spec 
+      (S.append (S.head (S.tail olds)) (S.head (S.tail hs))) (n - 1))
 
 // TODO: make a pure `exists` term for better elimination.
 val hash_ss_spec:
@@ -190,7 +243,7 @@ let hash_ss_spec_intro j n olds hs =
   exists_intro
     (fun (olds:hash_ss{S.length olds = n /\ hash_ss_length_spec j n olds hs}) ->
       hash_ss_spec_ j n olds hs) olds
-
+  
 // val hash_ss_spec_elim:
 //   j:nat -> n:nat{n > 0 && j <= pow2 n} ->
 //   hs:hash_ss{S.length hs = n} ->
@@ -209,6 +262,84 @@ let mt_wf_spec mt =
 
 /// Correctness of insertion
 
+private val seq_equal_slice_index:
+  #a:Type -> 
+  s1:S.seq a -> s2:S.seq a ->
+  n:nat -> m:nat{n <= m && m <= S.length s1 && m <= S.length s2} ->
+  i:nat{n <= i && i < m} ->
+  Lemma (requires (S.equal (S.slice s1 n m) (S.slice s2 n m)))
+        (ensures (S.index s1 i == S.index s2 i))
+private let seq_equal_slice_index #a s1 s2 n m i =
+  lemma_index_slice s1 n m (i - n);
+  lemma_index_slice s2 n m (i - n)
+
+private val seq_equal_slice_more:
+  #a:Type -> s1:S.seq a -> s2:S.seq a ->
+  n:nat -> m:nat{n <= m && m <= S.length s1 && m <= S.length s2} ->
+  k:nat{n <= k} -> l:nat{k <= l && l <= m} ->
+  Lemma (requires (S.equal (S.slice s1 n m) (S.slice s2 n m)))
+        (ensures (S.equal (S.slice s1 k l) (S.slice s2 k l)))
+private let seq_equal_slice_more #a s1 s2 n m k l =
+  slice_slice s1 n m (k - n) (l - n);
+  slice_slice s2 n m (k - n) (l - n)
+
+val hash_ss_insert_modified:
+  lv:nat{lv < 32} ->
+  i:nat ->
+  j:nat{i <= j /\ j < pow2 (32 - lv) - 1} ->
+  hs:hash_ss{S.length hs = 32 /\ hs_wf_elts lv hs i j} ->
+  v:hash ->
+  Lemma (S.equal (S.slice hs 0 lv)
+                 (S.slice (hash_ss_insert lv i j hs v) 0 lv) /\
+        S.equal (S.slice hs (lv + 1) 32)
+                 (S.slice (hash_ss_insert lv i j hs v) (lv + 1) 32) /\
+        S.equal (S.index (hash_ss_insert lv i j hs v) lv)
+                (S.snoc (S.index hs lv) v))
+let hash_ss_insert_modified lv i j hs v = ()
+
+val insert_modified:
+  lv:nat{lv < 32} ->
+  i:nat ->
+  j:nat{i <= j /\ j < pow2 (32 - lv) - 1} ->
+  hs:hash_ss{S.length hs = 32 /\ hs_wf_elts lv hs i j} ->
+  acc:hash ->
+  Lemma (requires True)
+        (ensures (S.equal (S.slice (insert_ lv i j hs acc) 0 lv)
+                          (S.slice hs 0 lv)))
+        (decreases j)
+let rec insert_modified lv i j hs acc =
+  let ihs = hash_ss_insert lv i j hs acc in
+  hash_ss_insert_modified lv i j hs acc;
+  if j % 2 = 1
+  then (let nacc = hash_2 (S.last (S.index hs lv)) acc in
+       insert_modified (lv + 1) (i / 2) (j / 2) ihs nacc;
+       seq_equal_slice_more (insert_ (lv + 1) (i / 2) (j / 2) ihs nacc) ihs
+         0 (lv + 1) 0 lv)
+  else ()
+
+val insert_head:
+  lv:nat{lv < 32} ->
+  i:nat ->
+  j:nat{i <= j /\ j < pow2 (32 - lv) - 1} ->
+  hs:hash_ss{S.length hs = 32 /\ hs_wf_elts lv hs i j} ->
+  acc:hash ->
+  Lemma (S.equal (S.index (insert_ lv i j hs acc) lv)
+                 (S.index (hash_ss_insert lv i j hs acc) lv))
+let insert_head lv i j hs acc =
+  if j % 2 = 1
+  then (let ihs = hash_ss_insert lv i j hs acc in
+       let nacc = hash_2 (S.last (S.index hs lv)) acc in
+       assert (S.equal (S.index (insert_ lv i j hs acc) lv)
+                       (S.index (insert_ (lv + 1) (i / 2) (j / 2) ihs nacc) lv));
+       insert_modified (lv + 1) (i / 2) (j / 2) ihs nacc;
+       assert (S.equal (S.slice (insert_ (lv + 1) (i / 2) (j / 2) ihs nacc) 0 (lv + 1))
+                       (S.slice ihs 0 (lv + 1)));
+       seq_equal_slice_index
+         (insert_ (lv + 1) (i / 2) (j / 2) ihs nacc) ihs
+         0 (lv + 1) lv
+  )
+  else ()
+
 val insert_wf_spec:
   lv:nat{lv < 32} ->
   i:nat ->
@@ -223,34 +354,38 @@ val insert_wf_spec:
                  hash_ss_spec_ (j + 1) (32 - lv) olds
                    (S.slice (insert_ lv i j hs acc) lv 32)))
         (decreases j)
-#reset-options "--z3rlimit 10 --max_fuel 1"
+#reset-options "--z3rlimit 20 --max_fuel 1"
 let rec insert_wf_spec lv i j hs acc olds =
   let ihs = insert_ lv i j hs acc in
+  insert_head lv i j hs acc;
+  hash_ss_insert_modified lv i j hs acc;
+  let spec_base = 
+    hash_seq_lift_to_spec
+      (S.append (S.head olds) (S.index hs lv)) (32 - lv) in
+
   if j % 2 = 1
   then begin
     remainder_2_1_div j;
-    // let nacc = hash_2 (S.last (S.index hs lv)) acc in
-    // insert_wf_spec (lv + 1) (i / 2) (j / 2) hs nacc (S.tail olds);
     admit ()
   end
+  
   else begin
     remainder_2_not_1_div j;
-    assert (S.equal (S.slice hs (lv + 1) 32) (S.slice ihs (lv + 1) 32));
-    let spec_base = hash_seq_lift_to_spec
-                      (S.append (S.head olds) (S.index hs lv)) (32 - lv) in
-    assert (hash_seq_spec_rel j (32 - lv) 
-             (S.head olds) (S.index hs lv) spec_base);
-    assert (hash_ss_spec_rel (j / 2) (32 - (lv + 1)) 
-             (S.tail olds) (S.slice hs (lv + 1) 32)
-             (mt_next_lv spec_base));
-    assert (hash_ss_spec_rel ((j + 1) / 2) (32 - (lv + 1)) 
-             (S.tail olds) (S.slice (insert_ lv i j hs acc) (lv + 1) 32)
-             (mt_next_lv spec_base));
-    let ispec_base = hash_seq_lift_to_spec
-                        (S.append (S.head olds) (S.index ihs lv)) (32 - lv) in
-    assume (hash_ss_spec_rel ((j + 1) / 2) (32 - (lv + 1)) 
-             (S.tail olds) (S.slice (insert_ lv i j hs acc) (lv + 1) 32)
-             (mt_next_lv ispec_base))
+    let ispec_base =
+      hash_seq_lift_to_spec
+        (S.append (S.head olds) (S.index ihs lv)) (32 - lv) in
+    // Since original `olds` and `hs[lv]` are unchanged after the insertion,
+    // below assertion holds.
+    assert (S.equal (S.slice (S.append (S.head olds) (S.index hs lv)) 0 j)
+                    (S.slice (S.append (S.head olds) (S.index ihs lv)) 0 j));
+    hash_seq_lift_to_spec_slice_eq
+      (S.append (S.head olds) (S.index hs lv))
+      (S.append (S.head olds) (S.index ihs lv))
+      (32 - lv) j;
+    mt_next_lv_equiv j (32 - lv) spec_base ispec_base;
+    hash_ss_spec_rel_equiv ((j + 1) / 2) (32 - (lv + 1))
+      (S.tail olds) (S.slice ihs (lv + 1) 32)
+      (mt_next_lv spec_base) (mt_next_lv ispec_base)
   end
 
 // val mt_insert_wf_spec_0:
